src/Bedrock/Synthesis/Examples/X1305_32.v
@@ -1,6 +1,7 @@
 Require Import Coq.ZArith.ZArith.
 Require Import Coq.Lists.List.
 Require Import Coq.Strings.String.
+Require Import Crypto.Bedrock.Parameters.SelectParameters.
 Require Import Crypto.Bedrock.Interfaces.UnsaturatedSolinas.
 Require Import Crypto.Bedrock.Synthesis.UnsaturatedSolinas.
 Local Open Scope Z_scope.
@@ -12,12 +13,19 @@ Let c := [(1, 5)].
 Let machine_wordsize := 32.
 Let prefix := "poly1305_"%string.
 
-Instance names : names_of_operations.
+Definition names : names_of_operations.
 make_names_of_operations prefix. Defined.
 
 Instance p : Types.parameters.
 make_parameters machine_wordsize. Defined.
 Instance p_ok : Types.ok. typeclasses eauto. Qed.
 
-Instance poly1305_bedrock2 : bedrock2_unsaturated_solinas n s c.
-Proof. make_bedrock2_unsaturated_solinas. Time Defined.
+Instance poly1305_bedrock2 : bedrock2_unsaturated_solinas.
+Proof.
+  let p := parameters_from_wordsize machine_wordsize in
+  make_bedrock2_unsaturated_solinas p names n s c machine_wordsize.
+Time Defined.
+(*
+Eval cbv [add poly1305_bedrock2] in add.
+Eval cbv [spec_of_add poly1305_bedrock2] in spec_of_add.
+*)
