src/Bedrock/Synthesis/UnsaturatedSolinas.v
@@ -19,7 +19,19 @@ Local Open Scope Z_scope.
 Import ListNotations.
 Import AbstractInterpretation.Compilers.
 
-Class bedrock2_unsaturated_solinas {p names n s c} :=
+Record names_of_operations :=
+  { name_of_carry_mul : string;
+    name_of_carry_square : string;
+    name_of_carry : string;
+    name_of_add : string;
+    name_of_sub : string;
+    name_of_opp : string;
+    name_of_selectznz : string;
+    name_of_to_bytes : string;
+    name_of_from_bytes : string;
+    name_of_carry_scmul_const : Z -> string }.
+
+Class bedrock2_unsaturated_solinas :=
   { carry_mul : bedrock_func;
     carry_square : bedrock_func;
     carry : bedrock_func;
@@ -29,24 +41,15 @@ Class bedrock2_unsaturated_solinas {p names n s c} :=
     selectznz : bedrock_func;
     to_bytes : bedrock_func;
     from_bytes : bedrock_func;
-    spec_of_carry_mul : spec_of (fst carry_mul) :=
-      @spec_of_carry_mul p n s c names;
-    spec_of_carry_square : spec_of (fst carry_square) :=
-      @spec_of_carry_square p n s c names;
-    spec_of_carry : spec_of (fst carry) :=
-      @spec_of_carry p n s c names;
-    spec_of_add : spec_of (fst add) :=
-      @spec_of_add p n s c names;
-    spec_of_sub : spec_of (fst sub) :=
-      @spec_of_sub p n s c names;
-    spec_of_opp : spec_of (fst opp) :=
-      @spec_of_opp p n s c names;
-    spec_of_selectznz : spec_of (fst selectznz) :=
-      @spec_of_selectznz p n s c names;
-    spec_of_to_bytes : spec_of (fst to_bytes) :=
-      @spec_of_to_bytes p n s c names;
-    spec_of_from_bytes : spec_of (fst from_bytes) :=
-      @spec_of_from_bytes p n s c names;
+    spec_of_carry_mul : spec_of (fst carry_mul);
+    spec_of_carry_square : spec_of (fst carry_square);
+    spec_of_carry : spec_of (fst carry);
+    spec_of_add : spec_of (fst add);
+    spec_of_sub : spec_of (fst sub);
+    spec_of_opp : spec_of (fst opp);
+    spec_of_selectznz : spec_of (fst selectznz);
+    spec_of_to_bytes : spec_of (fst to_bytes);
+    spec_of_from_bytes : spec_of (fst from_bytes);
     carry_mul_correct :
       forall functions,
         spec_of_carry_mul (carry_mul :: functions);
@@ -74,18 +77,34 @@ Class bedrock2_unsaturated_solinas {p names n s c} :=
     from_bytes_correct :
       forall functions,
         spec_of_from_bytes (from_bytes :: functions) }.
-Arguments bedrock2_unsaturated_solinas {_ _} _ _ _.
 
 (* scalar multiplication is calculated separately since it requires an extra
    argument *)
-Class bedrock2_unsaturated_solinas_scmul {p names n s c} {x : Z} :=
+Class bedrock2_unsaturated_solinas_scmul {x : Z} :=
   { carry_scmul_const : bedrock_func;
-    spec_of_carry_scmul_const : spec_of (fst carry_scmul_const) :=
-      @spec_of_carry_scmul_const p n s c names x;
+    spec_of_carry_scmul_const : spec_of (fst carry_scmul_const);
     carry_scmul_const_correct :
       forall functions,
         spec_of_carry_scmul_const (carry_scmul_const :: functions) }.
-Arguments bedrock2_unsaturated_solinas_scmul {_ _} _ _ _ _.
+Arguments bedrock2_unsaturated_solinas_scmul x : clear implicits.
+
+(*** Helpers ***)
+
+Definition names_from_prefix (prefix : string)
+  : names_of_operations :=
+  {| name_of_carry_mul := (prefix ++ "carry_mul")%string;
+     name_of_carry_square := (prefix ++ "carry_square")%string;
+     name_of_carry := (prefix ++ "carry")%string;
+     name_of_add := (prefix ++ "add")%string;
+     name_of_sub := (prefix ++ "sub")%string;
+     name_of_opp := (prefix ++ "opp")%string;
+     name_of_selectznz := (prefix ++ "selectznz")%string;
+     name_of_to_bytes := (prefix ++ "to_bytes")%string;
+     name_of_from_bytes := (prefix ++ "from_bytes")%string;
+     name_of_carry_scmul_const :=
+       fun x =>
+         (prefix ++ "carry_scmul_const" ++ Decimal.Z.to_string x)%string
+  |}.
 
 (*** Synthesis tactics ***)
 
@@ -93,8 +112,6 @@ Ltac handle_easy_preconditions :=
   lazymatch goal with
   | |- ZRange.type.option.is_tighter_than _ _ = true =>
     abstract (vm_compute; reflexivity)
-  | |- UnsaturatedSolinas.check_args _ _ _ _ _ = _ =>
-    abstract (native_compute; reflexivity)
   | |- Types.ok => solve [typeclasses eauto]
   | _ => first [ apply inname_gen_varname_gen_disjoint
                | apply outname_gen_varname_gen_disjoint
@@ -103,78 +120,107 @@ Ltac handle_easy_preconditions :=
   | |- ?g => fail "Unrecognized goal" g
   end.
 
-Ltac use_correctness_proofs :=
+Ltac use_correctness_proofs p n s c :=
+  let Hc := fresh in
   match goal with
-  | |- context [Interfaces.UnsaturatedSolinas.spec_of_carry_mul] =>
-    apply Interfaces.UnsaturatedSolinas.carry_mul_correct
-  | |- context [Interfaces.UnsaturatedSolinas.spec_of_carry_square] =>
-    apply Interfaces.UnsaturatedSolinas.carry_square_correct
-  | |- context [Interfaces.UnsaturatedSolinas.spec_of_carry] =>
-    apply Interfaces.UnsaturatedSolinas.carry_correct
-  | |- context [Interfaces.UnsaturatedSolinas.spec_of_add] =>
-    apply Interfaces.UnsaturatedSolinas.add_correct
-  | |- context [Interfaces.UnsaturatedSolinas.spec_of_sub] =>
-    apply Interfaces.UnsaturatedSolinas.sub_correct
-  | |- context [Interfaces.UnsaturatedSolinas.spec_of_opp] =>
-    apply Interfaces.UnsaturatedSolinas.opp_correct
-  | |- context [Interfaces.UnsaturatedSolinas.spec_of_selectznz] =>
-    apply Interfaces.UnsaturatedSolinas.selectznz_correct
-  | |- context [Interfaces.UnsaturatedSolinas.spec_of_to_bytes] =>
-    apply Interfaces.UnsaturatedSolinas.to_bytes_correct
-  | |- context [Interfaces.UnsaturatedSolinas.spec_of_from_bytes] =>
-    apply Interfaces.UnsaturatedSolinas.from_bytes_correct
-  | |- context [Interfaces.UnsaturatedSolinas.spec_of_carry_scmul_const] =>
-    apply Interfaces.UnsaturatedSolinas.carry_scmul_const_correct
+  | |- context [Interfaces.UnsaturatedSolinas.carry_mul] =>
+    apply (@Interfaces.UnsaturatedSolinas.carry_mul_correct
+             p default_inname_gen default_outname_gen n s c)
+  | |- context [Interfaces.UnsaturatedSolinas.carry_square] =>
+    apply (@Interfaces.UnsaturatedSolinas.carry_square_correct
+             p default_inname_gen default_outname_gen n s c)
+  | |- context [Interfaces.UnsaturatedSolinas.carry] =>
+    apply (@Interfaces.UnsaturatedSolinas.carry_correct
+             p default_inname_gen default_outname_gen n s c)
+  | |- context [Interfaces.UnsaturatedSolinas.add] =>
+    apply (@Interfaces.UnsaturatedSolinas.add_correct
+             p default_inname_gen default_outname_gen n s c)
+  | |- context [Interfaces.UnsaturatedSolinas.sub] =>
+    apply (@Interfaces.UnsaturatedSolinas.sub_correct
+             p default_inname_gen default_outname_gen n s c)
+  | |- context [Interfaces.UnsaturatedSolinas.opp] =>
+    apply (@Interfaces.UnsaturatedSolinas.opp_correct
+             p default_inname_gen default_outname_gen n s c)
+  | |- context [Interfaces.UnsaturatedSolinas.selectznz] =>
+    apply (@Interfaces.UnsaturatedSolinas.selectznz_correct
+             p default_inname_gen default_outname_gen n s c)
+  | |- context [Interfaces.UnsaturatedSolinas.to_bytes] =>
+    apply (@Interfaces.UnsaturatedSolinas.to_bytes_correct
+             p default_inname_gen default_outname_gen n s c)
+  | |- context [Interfaces.UnsaturatedSolinas.from_bytes] =>
+    apply (@Interfaces.UnsaturatedSolinas.from_bytes_correct
+             p default_inname_gen default_outname_gen n s c)
+  | |- context [Interfaces.UnsaturatedSolinas.carry_scmul_const] =>
+    apply (@Interfaces.UnsaturatedSolinas.carry_scmul_const_correct
+             p default_inname_gen default_outname_gen n s c)
   end.
 
-Ltac make_all_reified_ops n s c machine_wordsize :=
+Ltac make_all_reified_ops p names n s c machine_wordsize :=
+  let carry_mul_name := (eval compute in (name_of_carry_mul names)) in
+  let carry_square_name := (eval compute in (name_of_carry_square names)) in
+  let carry_name := (eval compute in (name_of_carry names)) in
+  let add_name := (eval compute in (name_of_add names)) in
+  let sub_name := (eval compute in (name_of_sub names)) in
+  let opp_name := (eval compute in (name_of_opp names)) in
+  let selectznz_name := (eval compute in (name_of_selectznz names)) in
+  let to_bytes_name := (eval compute in (name_of_to_bytes names)) in
+  let from_bytes_name := (eval compute in (name_of_from_bytes names)) in
   idtac "computing reified carry_mul (slow)...";
   make_reified_op
-    (Interfaces.UnsaturatedSolinas.carry_mul n s c)
+    p carry_mul_name
+    (@Interfaces.UnsaturatedSolinas.carry_mul p n s c)
     (PushButtonSynthesis.UnsaturatedSolinas.carry_mul
        n s c machine_wordsize);
   idtac "computing reified carry_square (slow)...";
   make_reified_op
-    (Interfaces.UnsaturatedSolinas.carry_square n s c)
+    p carry_square_name
+    (@Interfaces.UnsaturatedSolinas.carry_square p n s c)
     (PushButtonSynthesis.UnsaturatedSolinas.carry_square
        n s c machine_wordsize);
   idtac "computing reified carry...";
   make_reified_op
-    (Interfaces.UnsaturatedSolinas.carry n s c)
+    p carry_name
+    (@Interfaces.UnsaturatedSolinas.carry p n s c)
     (PushButtonSynthesis.UnsaturatedSolinas.carry
        n s c machine_wordsize);
   idtac "computing reified add...";
   make_reified_op
-    (Interfaces.UnsaturatedSolinas.add n s c)
+    p add_name
+    (@Interfaces.UnsaturatedSolinas.add p n s c)
     (PushButtonSynthesis.UnsaturatedSolinas.add
        n s c machine_wordsize);
   idtac "computing reified sub...";
   make_reified_op
-    (Interfaces.UnsaturatedSolinas.sub n s c)
+    p sub_name
+    (@Interfaces.UnsaturatedSolinas.sub p n s c)
     (PushButtonSynthesis.UnsaturatedSolinas.sub
        n s c machine_wordsize);
   idtac "computing reified opp...";
   make_reified_op
-    (Interfaces.UnsaturatedSolinas.opp n s c)
+    p opp_name
+    (@Interfaces.UnsaturatedSolinas.opp p n s c)
     (PushButtonSynthesis.UnsaturatedSolinas.opp
        n s c machine_wordsize);
   idtac "computing reified selectznz...";
   make_reified_op
-    (Interfaces.UnsaturatedSolinas.selectznz n s c)
+    p selectznz_name
+    (@Interfaces.UnsaturatedSolinas.selectznz p n s c)
     (PushButtonSynthesis.UnsaturatedSolinas.selectznz
        n machine_wordsize);
   idtac "computing reified to_bytes (slow)...";
   make_reified_op
-    (Interfaces.UnsaturatedSolinas.to_bytes n s c)
+    p to_bytes_name
+    (@Interfaces.UnsaturatedSolinas.to_bytes p n s c)
     (PushButtonSynthesis.UnsaturatedSolinas.to_bytes
        n s c machine_wordsize);
   idtac "computing reified from_bytes (slow)...";
   make_reified_op
-    (Interfaces.UnsaturatedSolinas.from_bytes n s c)
+    p from_bytes_name
+    (@Interfaces.UnsaturatedSolinas.from_bytes p n s c)
     (PushButtonSynthesis.UnsaturatedSolinas.from_bytes
        n s c machine_wordsize).
 
-Ltac instantiate_ops :=
+Ltac instantiate_ops p names n s c :=
   let carry_mul_func_value := fresh "carry_mul_func" in
   let carry_square_func_value := fresh "carry_square_func" in
   let carry_func_value := fresh "carry_func" in
@@ -185,7 +231,7 @@ Ltac instantiate_ops :=
   let to_bytes_func_value := fresh "to_bytes_func" in
   let from_bytes_func_value := fresh "from_bytes_func" in
   repeat match goal with
-         | X : reified_op ?op _ |- _ =>
+         | X : reified_op _ ?op _ |- _ =>
            lazymatch op with
            | context [Interfaces.UnsaturatedSolinas.carry_mul] =>
              destruct X as [? carry_mul_func_value ?]
@@ -207,43 +253,143 @@ Ltac instantiate_ops :=
              destruct X as [? from_bytes_func_value ?]
            end
          end;
-  apply Build_bedrock2_unsaturated_solinas
-    with (carry_mul:=carry_mul_func_value)
-         (carry_square:=carry_square_func_value)
-         (carry:=carry_func_value)
-         (add:=add_func_value)
-         (sub:=sub_func_value)
-         (opp:=opp_func_value)
-         (selectznz:=selectznz_func_value)
-         (to_bytes:=to_bytes_func_value)
-         (from_bytes:=from_bytes_func_value);
+  let carry_mul_name := (eval compute in (name_of_carry_mul names)) in
+  let carry_square_name := (eval compute in (name_of_carry_square names)) in
+  let carry_name := (eval compute in (name_of_carry names)) in
+  let add_name := (eval compute in (name_of_add names)) in
+  let sub_name := (eval compute in (name_of_sub names)) in
+  let opp_name := (eval compute in (name_of_opp names)) in
+  let selectznz_name := (eval compute in (name_of_selectznz names)) in
+  let to_bytes_name := (eval compute in (name_of_to_bytes names)) in
+  let from_bytes_name := (eval compute in (name_of_from_bytes names)) in
+    let carry_mul_spec :=
+        (eval cbv
+              [fst snd precondition postcondition
+                   Interfaces.UnsaturatedSolinas.carry_mul
+                   Interfaces.UnsaturatedSolinas.spec_of_carry_mul] in
+            (@Interfaces.UnsaturatedSolinas.spec_of_carry_mul
+               p n s c carry_mul_name)) in
+    let carry_square_spec :=
+        (eval cbv
+              [fst snd precondition postcondition
+                   Interfaces.UnsaturatedSolinas.carry_square
+                   Interfaces.UnsaturatedSolinas.spec_of_carry_square] in
+            (@Interfaces.UnsaturatedSolinas.spec_of_carry_square
+               p n s c carry_square_name)) in
+    let carry_spec :=
+        (eval cbv
+              [fst snd precondition postcondition
+                   Interfaces.UnsaturatedSolinas.carry
+                   Interfaces.UnsaturatedSolinas.spec_of_carry] in
+            (@Interfaces.UnsaturatedSolinas.spec_of_carry
+               p n s c carry_name)) in
+    let add_spec :=
+        (eval cbv
+              [fst snd precondition postcondition
+                   Interfaces.UnsaturatedSolinas.add
+                   Interfaces.UnsaturatedSolinas.spec_of_add] in
+            (@Interfaces.UnsaturatedSolinas.spec_of_add
+               p n s c add_name)) in
+    let sub_spec :=
+        (eval cbv
+              [fst snd precondition postcondition
+                   Interfaces.UnsaturatedSolinas.sub
+                   Interfaces.UnsaturatedSolinas.spec_of_sub] in
+            (@Interfaces.UnsaturatedSolinas.spec_of_sub
+               p n s c sub_name)) in
+    let opp_spec :=
+        (eval cbv
+              [fst snd precondition postcondition
+                   Interfaces.UnsaturatedSolinas.opp
+                   Interfaces.UnsaturatedSolinas.spec_of_opp] in
+            (@Interfaces.UnsaturatedSolinas.spec_of_opp
+               p n s c opp_name)) in
+    let selectznz_spec :=
+        (eval cbv
+              [fst snd precondition postcondition
+                   Interfaces.UnsaturatedSolinas.selectznz
+                   Interfaces.UnsaturatedSolinas.spec_of_selectznz] in
+            (@Interfaces.UnsaturatedSolinas.spec_of_selectznz
+               p n s c selectznz_name)) in
+    let to_bytes_spec :=
+        (eval cbv
+              [fst snd precondition postcondition
+                   Interfaces.UnsaturatedSolinas.to_bytes
+                   Interfaces.UnsaturatedSolinas.spec_of_to_bytes] in
+            (@Interfaces.UnsaturatedSolinas.spec_of_to_bytes
+               p n s c to_bytes_name)) in
+    let from_bytes_spec :=
+        (eval cbv
+              [fst snd precondition postcondition
+                   Interfaces.UnsaturatedSolinas.from_bytes
+                   Interfaces.UnsaturatedSolinas.spec_of_from_bytes] in
+            (@Interfaces.UnsaturatedSolinas.spec_of_from_bytes
+               p n s c from_bytes_name)) in
+    apply Build_bedrock2_unsaturated_solinas
+      with (carry_mul:=carry_mul_func_value)
+           (spec_of_carry_mul:=carry_mul_spec)
+           (carry_square:=carry_square_func_value)
+           (spec_of_carry_square:=carry_square_spec)
+           (carry:=carry_func_value)
+           (spec_of_carry:=carry_spec)
+           (add:=add_func_value)
+           (spec_of_add:=add_spec)
+           (sub:=sub_func_value)
+           (spec_of_sub:=sub_spec)
+           (opp:=opp_func_value)
+           (spec_of_opp:=opp_spec)
+           (selectznz:=selectznz_func_value)
+           (spec_of_selectznz:=selectznz_spec)
+           (to_bytes:=to_bytes_func_value)
+           (spec_of_to_bytes:=to_bytes_spec)
+           (from_bytes:=from_bytes_func_value)
+           (spec_of_from_bytes:=from_bytes_spec);
   subst carry_mul_func_value carry_square_func_value carry_func_value
         add_func_value sub_func_value opp_func_value selectznz_func_value
         to_bytes_func_value from_bytes_func_value.
 
-Ltac make_bedrock2_unsaturated_solinas :=
+Ltac make_bedrock2_unsaturated_solinas p names n s c machine_wordsize :=
+  assert (UnsaturatedSolinas.check_args
+            n s c machine_wordsize (ErrorT.Success tt) =
+          ErrorT.Success tt) by abstract (native_compute; reflexivity);
   match goal with
-    | |- @bedrock2_unsaturated_solinas ?p _ ?n ?s ?c =>
-      make_all_reified_ops n s c (@Semantics.width (@Types.semantics p));
-      instantiate_ops; use_correctness_proofs; try assumption;
+    | |- bedrock2_unsaturated_solinas =>
+      make_all_reified_ops p names n s c machine_wordsize;
+      instantiate_ops p names n s c;
+      use_correctness_proofs p n s c; try assumption;
       abstract (handle_easy_preconditions)
   end.
 
-Ltac make_bedrock2_unsaturated_solinas_scmul :=
-  match goal with
-    |- @bedrock2_unsaturated_solinas_scmul ?p _ ?n ?s ?c ?x =>
-    make_reified_op
-      (Interfaces.UnsaturatedSolinas.carry_scmul_const n s c x)
-      (PushButtonSynthesis.UnsaturatedSolinas.carry_scmul_const
-         n s c (@Semantics.width (@Types.semantics p)) x)
-  end;
+Ltac make_bedrock2_unsaturated_solinas_scmul
+     p names n s c machine_wordsize :=
+  assert (UnsaturatedSolinas.check_args
+            n s c machine_wordsize (ErrorT.Success tt) =
+          ErrorT.Success tt) by abstract (native_compute; reflexivity);
+  let x := match goal with
+             |- bedrock2_unsaturated_solinas_scmul ?x => x end in
+  let carry_scmul_const_name :=
+      (eval compute in (name_of_carry_scmul_const names x)) in
+  make_reified_op
+    p carry_scmul_const_name
+    (@Interfaces.UnsaturatedSolinas.carry_scmul_const p n s c x)
+    (PushButtonSynthesis.UnsaturatedSolinas.carry_scmul_const
+       n s c machine_wordsize x);
   let scmul_func_value := fresh "scmul_func_value" in
   match goal with
-  | X : reified_op ?op _ |- _ =>
+  | X : reified_op _ ?op _ |- _ =>
     destruct X as [? scmul_func_value ?] end;
+  let carry_scmul_const_spec :=
+      (eval cbv
+            [fst snd precondition postcondition
+                 Interfaces.UnsaturatedSolinas.carry_scmul_const
+                 Interfaces.UnsaturatedSolinas.spec_of_carry_scmul_const] in
+          (@Interfaces.UnsaturatedSolinas.spec_of_carry_scmul_const
+             p n s c x carry_scmul_const_name)) in
   apply Build_bedrock2_unsaturated_solinas_scmul
-    with (carry_scmul_const:=scmul_func_value); subst scmul_func_value;
-  use_correctness_proofs; try assumption;
+    with (carry_scmul_const:=scmul_func_value)
+         (spec_of_carry_scmul_const:=carry_scmul_const_spec);
+  subst scmul_func_value;
+  use_correctness_proofs p n s c; try assumption;
   abstract (handle_easy_preconditions).
 
 Ltac make_names_of_operations prefix :=
@@ -259,3 +405,28 @@ Ltac make_parameters machine_wordsize :=
     let p := parameters_from_wordsize machine_wordsize in
     exact p
   end.
+
+(*
+
+Let n := 5%nat.
+Let s := 2^130.
+Let c := [(1, 5)].
+Let machine_wordsize := 64.
+Let prefix := "poly1305_"%string.
+
+Definition names : names_of_operations.
+make_names_of_operations prefix. Defined.
+
+Instance poly1305_bedrock2 : bedrock2_unsaturated_solinas.
+Proof.
+  let p := parameters_from_wordsize machine_wordsize in
+  make_bedrock2_unsaturated_solinas p names n s c machine_wordsize.
+Time Defined.
+
+Instance poly1305_bedrock2_scmul5 : bedrock2_unsaturated_solinas_scmul 5.
+Proof.
+  let p := parameters_from_wordsize machine_wordsize in
+  make_bedrock2_unsaturated_solinas_scmul p names n s c machine_wordsize.
+Time Defined.
+
+*)
